src/phase0/helpers.dfy
@@ -1,0 +1,39 @@
+include "ssz.dfy"
+include "simpletypes.dfy"
+include "classes.dfy"
+include "consts.dfy"
+
+import opened SSZ
+import opened SimpleTypes
+import opened Classes
+import opened Consts
+
+predicate valid_constants() {
+  SECONDS_PER_SLOT != 0
+  && SLOTS_PER_EPOCH != 0
+  && INTERVALS_PER_SLOT != 0
+}
+
+predicate valid_time_slots(store: Store)
+  reads store
+{
+  store.time >= store.genesis_time
+}
+
+predicate valid_time_pure(store: Store_dt) {
+  store.time >= store.genesis_time
+}
+
+predicate valid_blocks(blocks: Dict<Root, BeaconBlock>)
+  reads blocks, blocks.values()
+{
+  valid_blocks_pure(blocks.repr)
+}
+
+predicate valid_blocks_pure(blocks: map<Root, BeaconBlock>)
+  reads blocks.Values
+{
+  forall r :: r in blocks.Keys ==>
+    var b := blocks[r];
+    b.slot == 0 || (b.parent_root in blocks.Keys && blocks[b.parent_root].slot < b.slot)
+}
